Lifter/Velocity/Auto_Lifter_Sets.thy
@@ -520,6 +520,12 @@ definition schem_lift_S_recL ::
     SP s1l s1r \<Rightarrow> (\<lambda> syn . (recl s1l s2) syn \<inter> (recr s1r s2) syn))"
 (*(\<lambda> syn . (recl s1l s2) syn \<inter> (recr s1r s2) syn)*)
 
+definition schem_lift_S_inject ::
+  " ('n, ('x, 'a, 'b, 'n) sinject, 'x, 'b) schem_lift_S" where
+"schem_lift_S_inject n s =
+  (case s of
+    SINJ _ S ls \<Rightarrow> S)"
+
 
 adhoc_overloading schem_lift_S
 
@@ -602,5 +608,7 @@ adhoc_overloading schem_lift_S
 "schem_lift_S_merge_recR_K_right schem_lift_S"
 
 "schem_lift_S_recL schem_lift_S schem_lift_S"
+
+schem_lift_S_inject
 
 end
