Lifter/Instances/Lift_Triv.thy
@@ -6,53 +6,88 @@ begin
 (*
  * triv
  *)
+(* we are revisiting this because automation seems to be having
+ * problems with triv in the presence of certain kinds of polymorphism.
+ * i wonder if we need an explicit type paramete?
+ *)
 definition triv_l ::
   "('x, 'a :: Bogus, 'a md_triv) lifting" where
 "triv_l =
   LMake (\<lambda> s a _ . mdt a) (\<lambda> s b . (case b of (mdt b') \<Rightarrow> b')) (\<lambda> s . mdt bogus)"
 
-interpretation triv_l : 
-  lifting_valid_weak "(triv_l :: ('x, 'a :: Bogus, 'a md_triv) lifting)" "\<lambda> _ . UNIV"
+locale triv_l_valid_weak =
+  fixes T :: "('a :: Bogus) itself"
+
+sublocale triv_l_valid_weak \<subseteq>
+  out : lifting_valid_weak "triv_l :: ('b, 'a, 'a md_triv) lifting" "(\<lambda> _ . UNIV)"
 proof
-  fix s :: 'x
-  fix a :: 'a
-  fix b
+  fix s :: 'b
+  fix a :: "'a :: Bogus"
+  fix b :: "'a md_triv"
   show "LOut (triv_l) s (LUpd (triv_l) s a b) = a"
     by(auto simp add:triv_l_def split:md_triv.splits)
 next
-  fix s :: 'x
+  fix s :: 'b
   fix b :: "'a md_triv"
 
   show "b <[ LUpd triv_l s (LOut triv_l s b) b"
    by(auto simp add:triv_l_def triv_pleq
           split:md_triv.splits)
 next
-  fix s :: 'x
+  fix s :: 'b
   fix a :: "'a"
   fix b :: "'a md_triv"
   show "LUpd triv_l s a b \<in> UNIV" by auto
 qed
 
+lemma (in triv_l_valid_weak) ax :
+  shows "lifting_valid_weak (triv_l :: ('b, 'a, 'a md_triv) lifting) (\<lambda> _ :: 'b . UNIV)"
+  using out.lifting_valid_weak_axioms
+  by auto
 
-interpretation triv_l:
-  lifting_valid_ok_ext "(triv_l :: ('x, 'a :: {Bogus, Okay}, 'a md_triv) lifting')" "\<lambda> _ . UNIV"
+lemma (in triv_l_valid_weak) ax_g :
+  assumes "S' = (\<lambda> _ . UNIV)"
+  shows "lifting_valid_weak (triv_l :: ('b, 'a, 'a md_triv) lifting) S'"
+  using out.lifting_valid_weak_axioms assms
+  by auto
+
+locale triv_l_valid_ok_ext =
+  fixes T :: "('a :: Bogus) itself"
+
+sublocale triv_l_valid_ok_ext \<subseteq>
+  out : lifting_valid_ok_ext "(triv_l :: ('b, 'a, 'a md_triv) lifting)" "(\<lambda> _ :: 'b . UNIV)"
 proof
   show "\<And> S . ok_S \<subseteq> UNIV" by auto
 next
-  fix s a b
+  fix s :: 'b
+  fix a :: 'a
+  fix b :: "'a md_triv"
   show "b \<in> ok_S \<Longrightarrow> LUpd triv_l s a b \<in> ok_S"
     by(auto simp add: triv_l_def triv_ok_S)
 qed
 
+lemma (in triv_l_valid_ok_ext) ax :
+  shows "lifting_valid_ok_ext (triv_l :: ('b, 'a, 'a md_triv) lifting) (\<lambda> _ :: 'b . UNIV)"
+  using out.lifting_valid_ok_ext_axioms
+  by auto
 
-interpretation triv_l :
-  lifting_valid_pres_ext "(triv_l :: ('x, 'a :: {Bogus}, 'a md_triv) lifting')" "\<lambda> _ . UNIV"
+lemma (in triv_l_valid_ok_ext) ax_g :
+  assumes "S' = (\<lambda> _ . UNIV)"
+  shows "lifting_valid_ok_ext (triv_l :: ('b, 'a, 'a md_triv) lifting) S'"
+  using assms out.lifting_valid_ok_ext_axioms
+  by auto
+
+locale triv_l_valid_pres_ext =
+  fixes T :: "('a :: Bogus) itself"
+
+sublocale triv_l_valid_pres_ext \<subseteq>
+  out : lifting_valid_pres_ext "(triv_l :: ('b, 'a, 'a md_triv) lifting)" "\<lambda> (_ :: 'b) . UNIV"
+
 proof
-next
   fix v :: "'a md_triv"
-  fix V 
+  fix V :: "'a md_triv set"
   fix supr :: "'a md_triv"
-  fix s 
+  fix s :: 'b
   fix f
 
   assume Nemp : "v \<in> V"
@@ -103,7 +138,22 @@ next
   qed
 qed
 
-interpretation triv_l : lifting_valid_pairwise_ext "\<lambda> _ . (UNIV :: 'a md_triv set)"
+lemma (in triv_l_valid_pres_ext) ax :
+  shows "lifting_valid_pres_ext (triv_l :: ('b, 'a, 'a md_triv) lifting) (\<lambda> _ . UNIV)"
+  using out.lifting_valid_pres_ext_axioms
+  by auto
+
+lemma (in triv_l_valid_pres_ext) ax_g :
+  assumes "S' = (\<lambda> _ . UNIV)"
+  shows "lifting_valid_pres_ext (triv_l :: ('b, 'a, 'a md_triv) lifting) S'"
+  using assms out.lifting_valid_pres_ext_axioms
+  by auto
+
+locale triv_l_valid_pairwise_ext =
+  fixes T :: "'a itself"
+
+sublocale triv_l_valid_pairwise_ext \<subseteq>
+  out : lifting_valid_pairwise_ext "\<lambda> (_ :: 'b) . (UNIV :: 'a md_triv set)"
 proof
   fix x1 x2 x3 s12 s23 s13 s123 :: "'a md_triv"
 
@@ -111,11 +161,26 @@ proof
     by auto
 qed
 
-interpretation triv_l : lifting_valid_oc_ext "triv_l ::('x, 'a :: {Bogus}, 'a md_triv) lifting'" "\<lambda> _ . (UNIV :: 'a md_triv set)"
+lemma (in triv_l_valid_pairwise_ext) ax :
+  shows "lifting_valid_pairwise_ext (\<lambda> (_ :: 'b) . (UNIV :: 'a md_triv set))"
+  using out.lifting_valid_pairwise_ext_axioms
+  by auto
+
+lemma (in triv_l_valid_pairwise_ext) ax_g :
+  assumes "S' = (\<lambda> (_ :: 'b) . (UNIV :: 'a md_triv set))"
+  shows "lifting_valid_pairwise_ext S'"
+  using assms out.lifting_valid_pairwise_ext_axioms
+  by auto
+
+locale triv_l_valid_oc_ext =
+  fixes T :: "('a :: Bogus) itself"
+
+sublocale triv_l_valid_oc_ext \<subseteq>
+  out: lifting_valid_oc_ext "(triv_l :: ('b, 'a, 'a md_triv) lifting)" "\<lambda> (_ :: 'b) . (UNIV :: 'a md_triv set)"
 proof
   fix x2 Xs 
   fix supr :: "'a md_triv" 
-  fix s :: 'x
+  fix s :: 'b
   fix r :: 'a
   fix w :: "'a md_triv"
   assume W: "w \<in> Xs"
@@ -136,5 +201,10 @@ proof
     using Supr_W
     by(auto simp add: triv_l_def)
 qed
+
+lemma (in triv_l_valid_oc_ext) ax :
+  shows "lifting_valid_oc_ext (triv_l :: ('b, 'a, 'a md_triv) lifting)"
+  using out.lifting_valid_oc_ext_axioms
+  by auto
 
 end
